DP progress and confusing isolated example

dp.dfy
@@ -4,92 +4,165 @@ method pick(max: int) returns (result: int)
 {
   assume false;
 }
-
-predicate inv(st: int, lfork: int, rfork: int)
+predicate inv2(st: int, lfork: int, rfork: int)
 {
   0<=st<=2 && 0<=lfork<=2 && 0<=rfork<=2 && !((st==2 && lfork==1 && rfork==1)||(st==2 && lfork==0 && rfork==1)||(st==2 && lfork==0 && rfork==0)||(st==2 && lfork==1 && rfork==0)||(st==2 && lfork==2 && rfork==1)||(st==2 && lfork==0 && rfork==2)||(st==2 && lfork==2 && rfork==2)||(st==2 && lfork==2 && rfork==0))
 }
 
-method step(phil: array<int>, fork: array<int>, n:int, i: int)
-    requires phil.Length==fork.Length==n
-    requires n>0
-    requires forall j:: 0<=j<n ==> inv(phil[j], fork[j], fork[(j+1)%n])
-    requires 0<=i<n && inv(phil[i], fork[i], fork[(i+1)%n])
-    ensures  0<=i<n && inv(phil[i], fork[i], fork[(i+1)%n])
-    ensures forall j:: 0<=j<n ==> inv(phil[j], fork[j], fork[(j+1)%n])
-    modifies phil
-    modifies fork
+predicate inv(st: int, lfork: int, rfork: int)
 {
-    if(phil[i]==0)
-    {
-      //Thinking->Hungry
-      phil[i] := 1;
-      assert phil[i]==2 ==> fork[i]==1;
-    }
-    else if (phil[i]==1)
-    {
-      //Hungry
-      if (fork[i]==1 && fork[(i+1) % n] ==2)
-      {
-        //Hungry->Eating
-        assert phil[i]==2 ==> fork[i]==1;
-        assert (fork[i]==1);
-        phil[i] := 2;
-        assert (fork[i]==1);
-        assert phil[i]==2 ==> fork[i]==1;
-      }
-      else
-      {
-        //Seek forks to pick up
-        var temp := pick(2);//try to pick up fork 0 or 1
-        if(temp==0)
-        {
-          //Try to pick up left fork
-          if(fork[i]==0)
-          {
-            fork[i] := 1;
-          }
-        }
-        else
-        {
-          //Try to pick up right fork
-          if(fork[(i+1)%n]==0)
-          {
-            fork[(i+1)%n] := 2;
-          }
-        }//end fork pick-up selection
-        assert phil[i]==2 ==> fork[i]==1;
-      }//end hungry but not all forks
-      assert phil[i]==2 ==> fork[i]==1;
-    }//end hungry
-    else
-    {
-      //Eating->Thinking
-      fork[i] := 0;
-      fork[(i+1)%n] := 0;
-      phil[i] := 0;
-      assert phil[i]==2 ==> fork[i]==1;
-    }
-    assert forall j:: 0<=j<n ==> inv(phil[j], fork[j], fork[(j+1)%n]);
+  0<=st<=2 && 0<=lfork<=2 && 0<=rfork<=2 && (st==2 ==> lfork==1) && (st==2 ==> rfork==2)
 }
 
-method Main(phil: array<int>, fork: array<int>, n: int) 
-  requires forall i:: 0<=i<phil.Length ==> phil[i] == 0
-  requires forall i:: 0<=i<fork.Length ==> fork[i] == 0
-  requires phil.Length == fork.Length ==n
-  requires n > 0
+lemma claim()
+{
+  assert forall i,j,k: int:: inv(i,j,k) <==> inv2(i,j,k);
+}
+
+lemma mod1()
+  ensures forall i,n: int:: 0<=i<n ==> (((i-1)%n)+1)%n == i
+{
+  assert forall i,n: int:: 0<=i<n ==> (((i-1)%n)+1)%n == i;
+}
+
+lemma mod2()
+  ensures forall i,n: int:: 0<=i<n ==> (((i+1)%n)+1)%n == (i+2)%n;
+{
+  assert forall i,n: int:: 0<=i<n ==> (((i+1)%n)+1)%n == (i+2)%n;
+}
+
+lemma mod3()
+  ensures forall n: int:: n>2 ==> (0+1)%n==1
+{
+  assert forall n: int:: n>2 ==> (0+1)%n==1;
+}
+
+lemma mod4()
+  ensures forall i,n:: 1<i<n-1 ==> ((i+1)%n != 0 && (i+1)%n != 1)
+{
+  assert forall i,n:: 1<i<n-1 ==> (i+1)%n != 0;
+  assert forall i,n:: 1<i<n-1 ==> (i+1)%n != 1;
+}
+
+method step(phil: array<int>, fork: array<int>, n:int, i: int)
+  requires phil.Length==fork.Length==n
+  requires n > 2
+  requires 0<=i<n
+  requires fork!=phil
+  requires forall j:: 0<=j<n ==> inv(phil[j], fork[j], fork[(j+1)%n])
+  ensures forall j:: 0<=j<n ==>  inv(phil[j], fork[j], fork[(j+1)%n])
   modifies phil
   modifies fork
 {
-  var steps := pick(100);
-  while (steps>0)//phil[i] has access to fork[i] and fork[i+1] mod n
-    decreases steps
-    invariant forall i:: 0<=i<n ==> inv(phil[i], fork[i], fork[(i+1)%n])
+  if(phil[i]==0)
   {
-    steps := steps-1;
-    var i := pick(phil.Length);
-    step(phil, fork, n, i);//move the i'th philosopher
-    assert phil[i]==2 ==> fork[i]==1;
-    assert phil[i]==2 ==> fork[(i+1)%n]==2;
+    //Thinking->Hungry
+    phil[i] := 1;
+  }
+  else if (phil[i]==1)
+  {
+    //Hungry
+    if (fork[i]==1 && fork[(i+1) % n] ==2)
+    {
+      //Hungry->Eating
+      phil[i] := 2;
+    }
+    else
+    {
+      //Seek forks to pick up
+      var temp := pick(2);//try to pick up fork 0 or 1
+      if(temp==0)
+      {
+        //Try to pick up left fork
+        if(fork[i]==0)
+        {
+          fork[i] := 1;
+        }
+      }
+      else
+      {
+        //Try to pick up right fork
+        if(fork[(i+1)%n]==0)
+        {
+          fork[(i+1)%n] := 2;
+        }
+      }//end fork pick-up selection
+    }//end hungry but not all forks
+  }//end hungry
+  else
+  {
+    //Eating->Thinking
+    assert 0<=i<n;
+    //Remind Dafny the invariant holds on nearby processes, which is very restricting
+    assert forall j::0<=j<n ==> inv(phil[j], fork[j], fork[(j+1)%n]);
+    mod1();
+    mod2();
+    mod3();
+    mod4();
+    assert (((i+1)%n)+1)%n==(i+2)%n;
+    assert (((i-1)%n)+1)%n==i;
+    assert inv(phil[(i+1)%n], fork[(i+1)%n], fork[(i+2)%n]);
+    assert inv(phil[(i-1)%n], fork[(i-1)%n], fork[i]);
+    assert inv(phil[i], fork[i], fork[(i+1)%n]);
+    assert forall j:: 0<=j<n ==> inv(phil[j], fork[j], fork[(j+1)%n]);
+    assert forall k: int:: k>2 ==> (0+1)%k==1;
+    assert (0+1)%n == 1;
+    assert inv(phil[0], fork[0], fork[1]);
+    assert forall j:: 1<=j<=i-1 ==> 0<=j<n;
+    assert forall j:: 1<=j<=i-1 ==> inv(phil[j], fork[j], fork[(j+1)%n]);
+    assert forall j:: 1<=j<=i-1 ==> (inv(phil[j], fork[j], fork[(j+1)%n]) ==> (phil[j]==2 ==> fork[j]==1));
+    assert forall j,k,l:: inv(j,k,l) ==> 0<=j<=2;
+    assert forall j,k,l:: inv(j,k,l) ==> 0<=k<=2;
+    assert forall j,k,l:: inv(j,k,l) ==> 0<=l<=2;
+    assert forall j:: 1<=j<=i-1 ==> (inv(phil[j], fork[j], fork[(j+1)%n] ==> 0<=phil[j]<=2);
+    assert forall j:: 1<=j<=i-1 ==> 0<=phil[j]<=2;
+    assert forall j:: 1<=j<=i-1 ==> 0<=fork[j]<=2;
+    assert forall j:: 1<=j<=i-1 ==> 0<=fork[(j+1)%n]<=2;
+    assert forall j:: 1<=j<=i-1 ==> (phil[j]==2 ==> fork[j]==1);
+    assert forall j:: 1<=j<=i-1 ==> (phil[j]==2 ==> fork[(j+1)%n]==2);
+    fork[i] := 0;
+    fork[(i+1)%n] := 0;
+    phil[i] := 0;
+    assert 1<i<n-1 ==> old(phil[0])==phil[0];
+    assert 1<i<n-1 ==> (i+1)%n != 0;
+    assert 1<i<n-1 ==> (i+1)%n != 1;
+    assert 1<i<n-1 ==> old(fork[0])==fork[0];
+    assert 1<i<n-1 ==> old(fork[1])==fork[1];
+    assert 1<i<n-1 ==> (phil[0]==2 ==> fork[0]==1);
+    assert 1<i<n-1 ==> (phil[0]==2 ==> fork[1]==2);
+    assert 1<i<n-1 ==> (0<=phil[0]<=2);
+    assert 1<i<n-1 ==> (0<=fork[0]<=2);
+    assert 1<i<n-1 ==> (0<=fork[1]<=2);
+    assert 1<i<n-1 ==> inv(phil[0], fork[0], fork[1]);//if i isn't near P0 (i==n-1, 0, or 1), invariant stays
+    assert inv(phil[0], fork[0], fork[1]);
+    assert forall j:: 1<=j<=i-1 ==> (phil[j]==2 ==> fork[j]==1);
+    assert forall j:: 1<=j<=i-1 ==> (phil[j]==2 ==> fork[(j+1)%n]==2);
+    assert forall j:: 1<=j<=i-1 ==> inv(phil[j], fork[j], fork[(j+1)%n]);//should be non-interference
+    assert inv(phil[i], fork[i], fork[(i+1)%n]);
+    assert inv(phil[(i+1)%n], fork[(i+1)%n], fork[(i+2)%n]);
+    assert forall j:: i+1<j<n-1 ==> inv(phil[j], fork[j], fork[(j+1)%n]);
+    assert inv(phil[n-1], fork[n-1], fork[0]);
+    assert forall j:: 0<=j<n ==> (j==0 || 1<=j<=i-1 || j==i || j==i+1 || i+1<j<n-1 || j==n-1);//prove the following by cases
+    assert forall j:: 0<=j<n ==>  inv(phil[j], fork[j], fork[(j+1)%n]);
+  }//End internal state detection
+}//end step() method
+
+method Main(phil: array<int>, fork:array<int>, n:int)
+  modifies phil
+  modifies fork
+  requires fork!=phil
+  requires phil.Length==fork.Length==n
+  requires n>2
+  requires forall j:: 0<=j<n ==> phil[j] == 0
+  requires forall j:: 0<=j<n ==> fork[j] == 0
+{
+  var steps := pick(1000);
+  while(steps>0)
+    decreases steps
+    invariant forall j:: 0<=j<n ==> inv(phil[j], fork[j], fork[(j+1)%n])
+  {
+    steps := steps - 1;
+    var i := pick(n);
+    step(phil, fork, n, i);
   }
 }
