confusion.dfy
@@ -1,0 +1,26 @@
+predicate inv(i: int, j: int, k: int)
+{
+    inv2(i)
+}
+
+predicate inv2(i: int)
+{
+  0<=i<=2
+}
+
+method Main(phil: array<int>, a: array<int>, b: array<int>, i: int, n: int)
+  requires phil.Length==a.Length==b.Length==n
+  requires 0<=i<n
+  requires n>2 
+{
+  assume forall j:: 0<=j<n-1 ==> inv(phil[j], a[j+1], a[j]);
+  assert forall j:: 0<=j<n-1 ==> (inv(phil[j], a[j+1], a[j]) ==> inv2(phil[j]));
+  assert forall j:: 0<=j<n-1 ==> inv2(phil[j]);
+}
+
+//Making inv() a binary predicate verifies
+//Making inv() be in three distinct arrays verifies
+//Making inv() refer to concrete values in the second/third components verifies
+//Making inv() refer to the same values in second/third components verifies.
+
+//Why as written does it not verify?
